Adding Exponentiation, comments and fixes.

code/dafny/array_search.dfy
@@ -24,7 +24,7 @@ method has_sequential(a: array<int>, key: int) returns (ret: int)
     }
 
 // Functional version
-function sorted(a: array<int>, index: int): bool
+function sortedf(a: array<int>, index: int): bool
     requires a != null;
     requires index >= 0;
     requires index <= a.Length;
@@ -33,11 +33,11 @@ function sorted(a: array<int>, index: int): bool
     {
         index == a.Length ||
         index == a.Length - 1 ||
-        (a[index] < a[index + 1] && sorted(a, index + 1))
+        (a[index] < a[index + 1] && sortedf(a, index + 1))
     }
 
 // Predicate version
-predicate sorted2(a: array<int>)
+predicate sorted(a: array<int>)
     requires a != null
     reads a
     {
@@ -45,11 +45,10 @@ predicate sorted2(a: array<int>)
     }
 
 // Binary search - Not working.
-/*method has_binary(a: array<int>, key: int) returns (ret: int)
+method has_binary(a: array<int>, key: int) returns (ret: int)
     requires a != null
     requires a.Length > 0
-    //requires sorted(a, 0)
-    requires sorted2(a)
+    requires sorted(a)
     // result = 0 => key belongs elements(a)
     {
         var min, max, x: int;
@@ -58,11 +57,10 @@ predicate sorted2(a: array<int>)
         max := a.Length - 1;
         x := 0;
         while(max != min)
-        invariant 0 <= min <= x <= max < a.Length;
-        //decreases max - min;
+        //invariant 0 <= min <= x <= max < a.Length;
+        decreases max - min;
         {
             x := (max + min) / 2;
-            assert(min <= x <= max);
             if a[x] < key {
                 min := x + 1;
             } else {
@@ -70,4 +68,4 @@ predicate sorted2(a: array<int>)
             }
             ret := min;
         }
-    }*/
+    }
