code/dafny/exponentiation.dfy
@@ -1,0 +1,39 @@
+// Common power method
+function method pow(a: int, b: int): int
+    requires b >= 0
+    {
+        if b == 0 then 1
+        else if b == 1 then a
+        else a * pow(a, b - 1)
+    }
+
+// Exponentiation by successive squaring.
+method power_binary(a: int, b: int) returns (ret: int)
+    requires b >= 0
+    // TODO Check
+    // ensures ret == pow(a, b)
+    {
+        // Init
+        var x, y: int;
+        ret := 1;
+        x := a;
+        y := b;
+
+        while (y != 0)
+        invariant  y >= 0
+        //TODO check invariant
+        //invariant  ret * pow(x, y) == pow(a, b)
+        decreases y
+        {
+          if (y % 2 == 0)
+          {
+             x := x * x;
+             y := y / 2;
+          }
+          else
+          {
+             ret := ret * x;
+             y := y - 1;
+          }
+        }
+    }
