code/dafny/gdc.dfy
@@ -1,3 +1,4 @@
+// Recursive GDC
 function gcd(m: int, n: int): int
     requires m > 0;
     requires n > 0;
@@ -8,7 +9,7 @@ function gcd(m: int, n: int): int
         else gcd(m, n-m) 
     }
 
-
+// GDC
 method gdc(a: int, b: int) returns (r: int)
     requires  a > 0  &&  b > 0;
     ensures r == gcd(a, b);
